src/3d/prelude/buffer/EverParse3d.Actions.All.fst
@@ -7,6 +7,6 @@ let ___PUINT8 = LowStar.Buffer.buffer FStar.UInt8.t
 
 let action_field_ptr
       #nz #wk (#k:Prelude.parser_kind nz wk) (#t:Type) (#p:Prelude.parser k t) (u:unit)
-   = fun input startPosition ->
+   = fun ctxt input startPosition ->
        let open LowParse.Slice in
        LowStar.Buffer.offset input.EverParse3d.InputStream.Buffer.Aux.buf startPosition
